VerusLean/VLIR/Elab.lean
@@ -63,7 +63,7 @@ def InequalityOp.toSyntax (i : InequalityOp) (lhs rhs : Term) : TermElabM Term :
 
 def UnaryOp.toSyntax (u : UnaryOp) (e : Term) : TermElabM Term := do
   match u with
-  | .Not => `(! ($e))
+  | .Not => `(¬ ($e))
   | .BitNot _ => `(~~~ $e)
   | .Trigger => `($e)
   | _ => throwError "unsupported unary op {repr u}"
@@ -101,10 +101,38 @@ partial def ExpX.toSyntax (e : ExpX) : TermElabM Term := do
   -- | .ArrayLiteral es =>
   --   let es ← es.mapM ExpX.toSyntax
   --   `(#[ $es,* ])
-  | .Bind (Bind.Quant q vars) e =>
-    -- let vs := vars.map Prod.fst
-    -- let ts := vars.map Prod.snd
-    let vars : TSyntaxArray ``Lean.Parser.Term.bracketedBinder ←
+
+  -- Call (fn : CallFun) (typs : List Typ) (exps : List ExpX)
+  | .Call fn typs exps =>
+    let fn := match fn with
+      | CallFun.Fun fn => fn.toSyntax
+    -- let typs ← typs.mapM Typ.toSyntax
+    let exps ← exps.mapM ExpX.toSyntax
+    let exps_TSepArray := exps.foldl Syntax.TSepArray.push (Syntax.TSepArray.mk #[] (sep := ","))
+    dbg_trace s!"elab get here!! {fn}, {exps}"
+    -- let termSyntaxList := exps.map (·.raw)
+    `($fn ( [$exps_TSepArray,*]) )
+    -- #check Syntax.TSepArray
+    -- let tupleSyntax := Syntax.node `Lean.Parser.Term.paren (#[mkAtom "(", mkSep "," termSyntaxList, mkAtom ")"])
+    -- mkParen (mkSep "," (terms.map exps))
+  | .Bind (Bind.Quant q vars) e => do
+    -- let xs := vars
+    -- vars.toArray.map (fun (i, ty) =>
+    --   let i := i.toSyntax
+    --   let ty ← ty.toSyntax
+    --   return (i, ty)
+    -- )
+    -- let vs := xs.map Prod.fst
+    -- let vs_syntax := Idents.toSyntax vs.toArray
+    -- let vs_tsyntax := vs_syntax.map TSyntax.mk
+    -- let ts := xs.map Prod.snd
+    -- let ts_syntax := (← ts.mapM Typ.toSyntax).toArray
+    -- let varsExists := Prod.mk vs_tsyntax ts_syntax
+    -- let varsExists := varsExists.mapM (fun (i, ty) =>
+    --   return (i, ty)
+    -- )
+
+    let varsForall : TSyntaxArray `Lean.Parser.Term.bracketedBinder ←
       (
         vars.toArray.mapM (fun (i, ty) => do
           let i := i.toSyntax
@@ -114,8 +142,17 @@ partial def ExpX.toSyntax (e : ExpX) : TermElabM Term := do
       )
     let e ← e.toSyntax
     match q with
-    | Quant.Forall => `(∀ $(vars):bracketedBinder*, $e)
-    | Quant.Exists => `(∀ $(vars):bracketedBinder*, $e)
+    | Quant.Forall => `(∀ $(varsForall):bracketedBinder*, $e)
+    | Quant.Exists => `(∀ $(varsForall):bracketedBinder*, $e)
+    -- | Quant.Exists =>  `(∃ $[($vs_tsyntax : $ts_syntax)]*, $e)
+    -- | Quant.Exists =>  `(∃ $vs_syntax:ident $ts_syntax:binderIdent*, $e)
+    -- | Quant.Exists => `(∃ $[$varsExists]*, $e)
+
+#check Exists
+#check Lean.Parser.Term.bracketedBinder
+-- #check Forall
+-- #check forall
+
 
 def Exps.toSyntax (e : Exps) : TermElabM (Array Term) := do
   e.mapM ExpX.toSyntax
@@ -140,5 +177,7 @@ def Decl.toSyntax (d : Decl) : CommandElabM (TSyntaxArray `command) := do
         := by sorry
     )
     return #[c]
+  | .specfn fnName inputTypes returnType body =>
+    throwError "specfn not supported"
 
 end VerusLean
